Isabelle2/AbstractMultiPaxosCorrectness.thy
@@ -6,7 +6,7 @@ imports AbstractMultiPaxos7 "../../IO-Automata/Simulations" "../../IO-Automata/I
 begin
 
 locale amp_proof = IOA + quorums quorums + amp_ioa quorums learners for 
-     quorums and learners :: "'l set" +
+     quorums :: "'a set set" and learners :: "'l set" +
   fixes the_ioa :: "(('v,'a)amp_state, ('v,'a,'l)amp_action) ioa"
   defines "the_ioa \<equiv> amp_ioa"
 begin
@@ -36,7 +36,8 @@ using assms by (auto split add:option.split_asm)
 subsection {* @{term conservative_array}  is an inductive invariant *}
 
 declare ballot_array.conservative_array_def[inv_proofs_defs]
-abbreviation conservative_array where 
+
+abbreviation conservative_array where
 "conservative_array s \<equiv>  \<forall> i . conservative_at s i"
 
 lemma conservative_inductive:
@@ -50,7 +51,7 @@ declare conservative_inductive[invs]
 
 subsection {* @{term safe}  is an inductive invariant *}
 
-abbreviation safe_at where "safe_at s i \<equiv> ballot_array.safe_at (ballot s) (vote s i) quorums"
+abbreviation safe_at where "safe_at s i \<equiv> ballot_array.safe_at  quorums (ballot s) (vote s i)"
 
 lemma trans_imp_prefix_order:
   assumes "s \<midarrow>a\<midarrow>the_ioa\<longrightarrow> t"
@@ -58,14 +59,15 @@ lemma trans_imp_prefix_order:
 by (cases a) (auto simp add:is_prefix_def inv_proofs_defs split add:option.split_asm)
     
 lemma safe_mono:
-  -- {* @{term safe_at} is monotonic. TODO: needed? *}
+  -- {* @{term safe_at} is monotonic. *}
   assumes "s \<midarrow>a\<midarrow>the_ioa\<longrightarrow> t" and "safe_at s i v b"
   shows "safe_at t i v b" using assms 
   by (drule_tac trans_imp_prefix_order)
-   (metis (full_types) assms(1) ballot_array_prefix.safe_at_mono ballot_array_prefix_def trans_imp_prefix_order)
+    (meson assms(1) ballot_array_prefix.safe_at_mono ballot_array_prefix_axioms_def ballot_array_prefix_def quorums_axioms trans_imp_prefix_order)
 
-abbreviation safe where "safe s \<equiv> \<forall> i . ballot_array.safe (ballot s) (vote s i) quorums"
+abbreviation safe where "safe s \<equiv> \<forall> i . ballot_array.safe  quorums (ballot s) (vote s i)"
 
+text {* TODO: make this proof generic to all algorithms in which the ballot array grows with safe_at values *}
 lemma safe_inv:
   "invariant the_ioa safe"
 apply (try_solve_inv2 inv_proofs_defs:inv_proofs_defs ballot_array.safe_def invs:invs)
@@ -83,17 +85,13 @@ proof (auto simp add:ballot_array.safe_def split add:option.splits)
     with prems(2) \<open>vote t i a b = Some v\<close> obtain q where "do_vote a i q v s t" and "ballot s a = b"
       apply(simp add:is_trans_def the_ioa_def amp_ioa_def amp_trans_def del:do_vote_def)
       apply(elim amp_trans_rel.elims)
-      apply simp
-      apply simp
-      defer
-      apply simp
-      apply (simp (no_asm_use))
+      apply simp apply simp defer apply simp
       apply (smt amp_ioa.do_vote_def amp_state.iffs amp_state.surjective amp_state.update_convs(3) fun_upd_apply option.sel)
       done
     hence "proved_safe_at s i q (ballot s a) v" and "q \<in> quorums" and "\<forall> a2 \<in> q . ballot s a \<le> ballot s a2" 
-      by (simp_all add:ballot_array.proved_safe_at_def split add:nat.splits)
+      by (auto simp add:ballot_array.proved_safe_at_2_def split add:nat.splits)
     hence "safe_at s i v b" using quorums_axioms prems(1) prems(3) `ballot s a = b`
-      ballot_array_props.proved_safe_at_imp_safe_at[of quorums "ballot s a" "vote s i" "ballot s" q v]
+      ballot_array_props.proved_safe_at_2_imp_safe_at[of quorums "ballot s a" "vote s i" "ballot s" q v]
       by (auto simp add:ballot_array.safe_def ballot_array_props_def split add:option.splits)
     thus "safe_at t i v b" using prems(2) safe_mono by simp
   qed
@@ -109,9 +107,7 @@ definition agreement where
 lemma agreement:"invariant the_ioa agreement"
 apply(rule invariantI)
     apply(auto simp add: inv_proofs_defs agreement_def ballot_array.chosen_def ballot_array.chosen_at_def)[1]
-    apply (metis empty_iff quorum_inter_witness)
-  apply instantiate_invs_2
-  apply (meson agreement_def ballot_array_props.intro ballot_array_props.safe_imp_agreement quorums_axioms)
+  apply (metis (mono_tags, lifting) IOA.invariant_def IOA.reachable_n agreement_def amp_proof.safe_inv amp_proof_axioms ballot_array_props.intro ballot_array_props.safe_imp_agreement quorums_axioms the_ioa_def)
 done
 
 end
