Isabelle2/LinorderOption.thy
@@ -34,7 +34,7 @@ done
 
 end
 
-instantiation option :: (linorder) linorder
+instantiation option :: (linorder) "{linorder,order_bot}"
 begin
 
 instance 
@@ -42,6 +42,7 @@ apply(intro_classes)
 apply (auto simp add:less_eq_def less_def)
 apply (metis less_eq_o.elims(2) option.inject option.simps(3) order_class.order.antisym)
 apply (metis le_cases less_eq_o.elims(3) less_eq_o.simps(3))
+apply (metis bot_def less_eq_o.simps(1))
 done
 
 end
